examples/lowparse/LowParse.Impl.VLBytes.Part5.fst
@@ -16,9 +16,9 @@ inline_for_extraction
 val point_to_vlbytes_contents
   (sz: integer_size)
   (f: (bounded_integer sz -> Tot bool))
-  (#b: bool)
+  (#k: parser_kind)
   (#t: Type0)
-  (p: parser' b t)
+  (p: parser k t)
   (b: S.bslice)
 : HST.Stack S.bslice
   (requires (fun h ->
@@ -29,9 +29,9 @@ val point_to_vlbytes_contents
     point_to_vlbytes_contents_postcond sz f p b h0 b'
   ))
 
-#set-options "--z3rlimit 16"
+#set-options "--z3rlimit 64"
 
-let point_to_vlbytes_contents sz f #b #t p b =
+let point_to_vlbytes_contents sz f #k #t p b =
   let h = HST.get () in
   let (len, _) = parse_bounded_integer_st_nochk sz b in
   let b1 = S.advance_slice b (U32.uint_to_t sz) in
@@ -42,14 +42,70 @@ let point_to_vlbytes_contents sz f #b #t p b =
 
 #reset-options
 
-#set-options "--z3rlimit 256"
+val serialize_vlbytes_gen_correct_aux
+  (sz: integer_size)
+  (f: (bounded_integer sz -> Tot bool))
+  (#k: parser_kind)
+  (#t: Type0)
+  (p: parser k t)
+  (b b1 b2: bytes32)
+: Lemma
+  (requires (
+    Seq.length b1 == sz /\ (
+    let vlen = parse (parse_bounded_integer sz) b1 in
+    Some? vlen /\ (
+    let (Some (len, _)) = vlen in
+    f len == true /\
+    Seq.length b2 == U32.v len /\ (
+    let vv = parse p b2 in
+    Some? vv /\ (
+    let (Some (_, consumed)) = vv in
+    consumed == Seq.length b2 /\
+    Seq.length b1 <= Seq.length b /\
+    Seq.slice b 0 (Seq.length b1) == b1 /\
+    Seq.slice b (Seq.length b1) (Seq.length b) == b2
+  ))))))
+  (ensures (
+    let vv = parse p b2 in
+    Some? vv /\ (
+    let (Some (v, consumed)) = vv in
+    let vv' = parse (parse_vlbytes_gen sz f p) b in
+    Some? vv' /\ (
+    let (Some (v', consumed')) = vv' in
+    v == v' /\
+    consumed == Seq.length b2 /\
+    consumed' == Seq.length b
+  ))))
+
+#set-options "--z3rlimit 64"
+
+let serialize_vlbytes_gen_correct_aux sz f #k #t p b b1 b2 =
+  let (Some (len, consumed1)) = parse (parse_bounded_integer sz) b1 in
+  assert (consumed1 == sz);
+  assert (no_lookahead_on (parse_bounded_integer sz) b1 b);
+  let v1' = parse (parse_bounded_integer sz) b in
+  assert (Some? v1');
+  let (Some (len', consumed1')) = v1' in
+  assert (consumed1' == sz);
+  assert (injective_postcond (parse_bounded_integer sz) b1 b);
+  assert (len' == len);
+  let v1_ = parse (parse_filter (parse_bounded_integer sz) f) b in
+  assert (Some? v1_);
+  let (Some (len_, consumed1_)) = v1_ in
+  assert (consumed1_ == sz);
+  assert ((len_ <: bounded_integer sz) == len);
+  ()
+
+#reset-options
+
+#set-options "--z3rlimit 16"
 
 let serialize_vlbytes_gen_correct
   (sz: integer_size)
   (f: (bounded_integer sz -> Tot bool))
-  (#b: bool)
+  (#k: parser_kind)
   (#t: Type0)
-  (p: parser' b t)
+  (p: parser k t)
   (b b1 b2: S.bslice)
   (h: HS.mem)
 : Lemma
@@ -66,64 +122,138 @@ let serialize_vlbytes_gen_correct
     exactly_parses h p b2 (fun v' ->
     v == v'
   ))))
-= assert (no_lookahead_on _ (parse_bounded_integer sz) (S.as_seq h b1) (S.as_seq h b));
-  assert (injective_postcond (parse_bounded_integer sz) (S.as_seq h b1) (S.as_seq h b))
+= let s = S.as_seq h b in
+  let s1 = S.as_seq h b1 in
+  let s2 = S.as_seq h b2 in
+  serialize_vlbytes_gen_correct_aux sz f p s s1 s2
 
 #reset-options
 
 module B = FStar.Buffer
 
-inline_for_extraction
-val serialize_bounded_integer_3
-  (i: bounded_integer 3)
-  (dest: S.bslice)
-: HST.Stack (S.bslice * S.bslice)
+let serialize_bounded_integer_t
+  (sz: integer_size)
+: Tot Type
+= (i: bounded_integer sz) ->
+  (dest: S.bslice) ->
+  HST.Stack (S.bslice * S.bslice)
   (requires (fun h ->
     S.live h dest /\
-    U32.v (S.length dest) >= 3
+    U32.v (S.length dest) >= sz
   ))
   (ensures (fun h (destl, destr) h' ->
     S.is_concat dest destl destr /\
-    U32.v (S.length destl) == 3 /\
+    U32.v (S.length destl) == sz /\
     S.live h' destr /\
     B.modifies_1 (S.as_buffer destl) h h' /\
-    exactly_parses h' parse_bounded_integer_3 destl (fun i' ->
+    exactly_parses h' (parse_bounded_integer' sz) destl (fun i' ->
     i' == i
   )))
 
-#set-options "--z3rlimit 128 --smtencoding.elim_box true --smtencoding.l_arith_repr native --smtencoding.nl_arith_repr native"
-
-let serialize_bounded_integer_3 i dest =
-  let h = HST.get () in
-  let lo = Cast.uint32_to_uint8 (U32.rem i 256ul) in
+let serialize_bounded_integer_3_unsynth
+  (i: bounded_integer 3)
+: Tot (U16.t * U8.t)
+= let lo = Cast.uint32_to_uint8 (U32.rem i 256ul) in
   let i' = U32.div i 256ul in
-  assert (U32.v i' < pow2 16);
-  assert (U32.v i' % pow2 16 == U32.v i');
   let hi = Cast.uint32_to_uint16 i' in
-  assert (i == U32.add (Cast.uint8_to_uint32 lo) (U32.mul 256ul (Cast.uint16_to_uint32 hi)));
-  let (dhi, d1) = serialize_u16 hi dest in
-  let h1 = HST.get () in
-  let (dlo, destr) = serialize_u8 lo d1 in
+  (hi, lo)
+
+#set-options "--z3rlimit 256 --smtencoding.elim_box true --smtencoding.l_arith_repr native --smtencoding.nl_arith_repr native"
+
+let serialize_bounded_integer_3_unsynth_correct
+  (i: bounded_integer 3)
+: Lemma
+  (parse_bounded_integer_3_synth (serialize_bounded_integer_3_unsynth i) == i)
+= ()
+
+#reset-options
+
+inline_for_extraction
+val serialize_bounded_integer_3
+: serialize_bounded_integer_t 3
+
+#set-options "--z3rlimit 64"
+
+let serialize_bounded_integer_3 = fun (i: bounded_integer 3) (dest: S.bslice) ->
+  let h = HST.get () in
   let destl = S.truncate_slice dest 3ul in
-  let f1 () : Lemma (S.is_concat destl dhi dlo) =
-    assert (dhi == S.truncated_slice destl 2ul);
-    assert (dlo == S.advanced_slice destl 2ul);
-    S.is_concat_intro destl 2ul
-  in
-  f1 ();
-  let f2 () : Lemma (S.is_concat dest destl destr) =
-    assert (destl == S.truncated_slice dest 3ul);
-    assert (destr == S.advanced_slice dest 3ul);
-    S.is_concat_intro dest 3ul
-  in
-  f2 ();
+  let destr = S.advance_slice dest 3ul in
+  let (hi, lo) = serialize_bounded_integer_3_unsynth i in
+  let (dhi, d1) = serialize_u16 hi destl in
+  let h1 = HST.get () in
+//  assert (exactly_parses h1 parse_u16 dhi (fun v1 -> v1 == hi));
+  let (dlo, _) = serialize_u8 lo d1 in
   let h' = HST.get () in
+  assert (dlo == d1);
+//  assert (exactly_parses h' parse_u8 dlo (fun v2 -> v2 == lo));
+  S.disjoint_truncated_slice_advanced_slice destl 2ul 2ul;
+  assert (S.disjoint dhi dlo);
   assert (S.as_seq h' dhi == S.as_seq h1 dhi);
+//  assert (exactly_parses h' parse_u16 dhi (fun v1 -> v1 == hi));
   serialize_nondep_then_correct parse_u16 parse_u8 destl dhi dlo h';
-  assert (B.modifies_1 (S.as_buffer destl) h h');
+//  assert (exactly_parses h' (nondep_then parse_u16 parse_u8) destl (fun v -> v == (hi, lo)));
+  parse_bounded_integer_3_synth_injective ();
+  serialize_synth_correct (nondep_then parse_u16 parse_u8) parse_bounded_integer_3_synth destl h';
+//  assert (exactly_parses h' parse_bounded_integer_3 destl (fun v -> v == parse_bounded_integer_3_synth (hi, lo)));
+  serialize_bounded_integer_3_unsynth_correct i;
   (destl, destr)
 
 #reset-options
+
+inline_for_extraction
+val serialize_bounded_integer_1
+: serialize_bounded_integer_t 1
+
+#set-options "--z3rlimit 16"
+
+let serialize_bounded_integer_1 = fun (i: bounded_integer 1) (dest: S.bslice) ->
+  assert (U32.v i < pow2 8);
+  assert (U32.v i % pow2 8 == U32.v i);
+  assert (Cast.uint8_to_uint32 (Cast.uint32_to_uint8 i) == i);
+  let (destl, destr) = serialize_u8 (Cast.uint32_to_uint8 i) dest in
+  let h = HST.get () in
+  serialize_synth_correct parse_u8 parse_bounded_integer_1_synth destl h;
+  (destl, destr)
+
+#reset-options
+
+inline_for_extraction
+val serialize_bounded_integer_2
+: serialize_bounded_integer_t 2
+
+#set-options "--z3rlimit 16"
+
+let serialize_bounded_integer_2 = fun (i: bounded_integer 2) (dest: S.bslice) ->
+  assert (U32.v i < pow2 16);
+  assert (U32.v i % pow2 16 == U32.v i);
+  assert (Cast.uint16_to_uint32 (Cast.uint32_to_uint16 i) == i);
+  let (destl, destr) = serialize_u16 (Cast.uint32_to_uint16 i) dest in
+  let h = HST.get () in
+  serialize_synth_correct parse_u16 parse_bounded_integer_2_synth destl h;
+  (destl, destr)
+
+#reset-options
+
+inline_for_extraction
+val serialize_bounded_integer_4
+: serialize_bounded_integer_t 4
+
+#set-options "--z3rlimit 16"
+
+let serialize_bounded_integer_4 = fun (i: bounded_integer 4) (dest: S.bslice) ->
+  serialize_u32 i dest
+
+#reset-options
+
+inline_for_extraction
+let serialize_bounded_integer'
+  (sz: integer_size)
+: Tot (serialize_bounded_integer_t sz)
+= match sz with
+  | 1 -> (serialize_bounded_integer_1 <: serialize_bounded_integer_t sz)
+  | 2 -> (serialize_bounded_integer_2 <: serialize_bounded_integer_t sz)
+  | 3 -> (serialize_bounded_integer_3 <: serialize_bounded_integer_t sz)
+  | 4 -> (serialize_bounded_integer_4 <: serialize_bounded_integer_t sz)
 
 inline_for_extraction
 val serialize_bounded_integer
@@ -144,31 +274,9 @@ val serialize_bounded_integer
     i' == i
   )))
 
-#set-options "--z3rlimit 16"
-
 let serialize_bounded_integer sz i dest =
   Classical.forall_intro (parse_bounded_integer'_correct sz);
-  match sz with
-  | 1 -> 
-    assert (U32.v i < pow2 8);
-    assert (U32.v i % pow2 8 == U32.v i);
-    assert (Cast.uint8_to_uint32 (Cast.uint32_to_uint8 i) == i);
-    let (destl, destr) = serialize_u8 (Cast.uint32_to_uint8 i) dest in
-    (destl, destr)
-  | 2 ->
-    assert (U32.v i < pow2 16);
-    assert (U32.v i % pow2 16 == U32.v i);
-    assert (Cast.uint16_to_uint32 (Cast.uint32_to_uint16 i) == i);
-    let (destl, destr) = serialize_u16 (Cast.uint32_to_uint16 i) dest in
-    (destl, destr)
-  | 4 ->
-    let (destl, destr) = serialize_u32 i dest in
-    (destl, destr)
-  | 3 ->
-    let (destl, destr) = serialize_bounded_integer_3 i dest in
-    (destl, destr)
-
-#reset-options
+  serialize_bounded_integer' sz i dest
 
 #set-options "--z3rlimit 16"
 
@@ -176,9 +284,9 @@ module B = FStar.Buffer
 
 inline_for_extraction
 val serialize_vlbytes_gen
-  (#b: bool)
+  (#k: parser_kind)
   (#t: Type0)
-  (p: parser' b t)
+  (p: parser k t)
   (sz: integer_size)
   (sz' : U32.t)
   (f: (bounded_integer sz -> Tot bool))
@@ -211,7 +319,7 @@ val serialize_vlbytes_gen
 
 #set-options "--z3rlimit 128 --smtencoding.elim_box true"
 
-let serialize_vlbytes_gen #b #t p sz sz' f src dest =
+let serialize_vlbytes_gen #k #t p sz sz' f src dest =
   let len = S.length src in
   let len' = U32.add sz' len in
   let destl = S.truncate_slice dest len' in
@@ -227,9 +335,9 @@ let serialize_vlbytes_gen #b #t p sz sz' f src dest =
 
 inline_for_extraction
 val serialize_vlbytes
-  (#b: bool)
+  (#k: parser_kind)
   (#t: Type0)
-  (p: parser' b t)
+  (p: parser k t)
   (sz: integer_size)
 : (src: S.bslice) ->
   (dest: S.bslice) ->
@@ -254,15 +362,15 @@ val serialize_vlbytes
     v == v' /\ v == v''
   )))))
   
-let serialize_vlbytes #b #t p sz =
+let serialize_vlbytes #k #t p sz =
   let sz' = U32.uint_to_t sz in
   serialize_vlbytes_gen p sz sz' (unconstrained_bounded_integer sz)
 
 inline_for_extraction
 val serialize_bounded_vlbytes
-  (#b: bool)
+  (#k: parser_kind)
   (#t: Type0)
-  (p: parser' b t)
+  (p: parser k t)
   (min: U32.t)
   (max: U32.t { U32.v max > 0 } )
 : (src: S.bslice) ->
@@ -291,7 +399,7 @@ val serialize_bounded_vlbytes
     v == v' /\ v == v''
   )))))
   
-let serialize_bounded_vlbytes #b #t p min max =
+let serialize_bounded_vlbytes #k #t p min max =
   let sz : integer_size = log256 max in
   let sz' : U32.t = U32.uint_to_t sz in
   serialize_vlbytes_gen p sz sz' (in_bounds min max)
