examples/lowparse/LowParse.Spec.Base.fst
@@ -33,7 +33,7 @@ let parse
 = p input
 
 let no_lookahead_weak_on
-  (t: Type0)
+  (#t: Type0)
   (f: bare_parser t)
   (x x' : bytes32)
 : GTot Type0
@@ -57,15 +57,15 @@ let no_lookahead_weak_on_ext
     parse f2 x' == parse f1 x'
   ))
   (ensures (
-    no_lookahead_weak_on _ f2 x x' <==> no_lookahead_weak_on _ f1 x x'
+    no_lookahead_weak_on f2 x x' <==> no_lookahead_weak_on f1 x x'
   ))
 = ()
 
 let no_lookahead_weak
-  (t: Type0)
+  (#t: Type0)
   (f: bare_parser t)
 : GTot Type0
-= forall (x x' : bytes32) . no_lookahead_weak_on t f x x'
+= forall (x x' : bytes32) . no_lookahead_weak_on f x x'
 
 let no_lookahead_weak_ext
   (#t: Type0)
@@ -75,7 +75,7 @@ let no_lookahead_weak_ext
     (forall (b: bytes32) . parse f2 b == parse f1 b)
   ))
   (ensures (
-    no_lookahead_weak t f2 <==> no_lookahead_weak t f1
+    no_lookahead_weak f2 <==> no_lookahead_weak f1
   ))
 = Classical.forall_intro_2 (fun b1 -> Classical.move_requires (no_lookahead_weak_on_ext f1 f2 b1))
 
@@ -153,7 +153,7 @@ let injective_ext
   Classical.forall_intro_2 (fun b1 -> Classical.move_requires (injective_postcond_ext p1 p2 b1))
   
 let no_lookahead_on_precond
-  (t: Type0)
+  (#t: Type0)
   (f: bare_parser t)
   (x x' : bytes32)
 : GTot Type0
@@ -165,7 +165,7 @@ let no_lookahead_on_precond
   )
 
 let no_lookahead_on_postcond
-  (t: Type0)
+  (#t: Type0)
   (f: bare_parser t)
   (x x' : bytes32)
 : GTot Type0
@@ -179,11 +179,11 @@ let no_lookahead_on_postcond
   ))
 
 let no_lookahead_on
-  (t: Type0)
+  (#t: Type0)
   (f: bare_parser t)
   (x x' : bytes32)
 : GTot Type0
-= no_lookahead_on_precond t f x x' ==> no_lookahead_on_postcond t f x x'
+= no_lookahead_on_precond f x x' ==> no_lookahead_on_postcond f x x'
 
 let no_lookahead_on_ext
   (#t: Type0)
@@ -195,15 +195,15 @@ let no_lookahead_on_ext
     parse p2 b2 == parse p1 b2
   ))
   (ensures (
-    no_lookahead_on _ p2 b1 b2 <==> no_lookahead_on _ p1 b1 b2
+    no_lookahead_on p2 b1 b2 <==> no_lookahead_on p1 b1 b2
   ))
 = ()
 
 let no_lookahead
-  (t: Type0)
+  (#t: Type0)
   (f: bare_parser t)
 : GTot Type0
-= forall (x x' : bytes32) . no_lookahead_on t f x x'
+= forall (x x' : bytes32) . no_lookahead_on f x x'
 
 let no_lookahead_ext
   (#t: Type0)
@@ -213,37 +213,9 @@ let no_lookahead_ext
     forall (b: bytes32) . parse p2 b == parse p1 b
   ))
   (ensures (
-    no_lookahead _ p2 <==> no_lookahead _ p1
+    no_lookahead p2 <==> no_lookahead p1
   ))
 = Classical.forall_intro_2 (fun b1 -> Classical.move_requires (no_lookahead_on_ext p1 p2 b1))
-
-let parser'
-  (b: bool)
-  (t: Type0)
-: Tot Type0
-= (f: bare_parser t { no_lookahead_weak t f /\ injective f /\ (if b then no_lookahead t f else True) } )
-
-let weak_parser (t: Type0) : Tot Type0 = parser' false t
-
-let parser (t: Type0) : Tot Type0 = parser' true t
-
-unfold
-let weaken (#t: Type0) (p: parser t) : Tot (weak_parser t) =
-  let p' : bare_parser t = p in (p' <: weak_parser t)
-
-unfold
-let weaken' (b: bool) (#t: Type0) (p: parser t) : Tot (parser' b t) =
-  let p' : bare_parser t = p in (p' <: parser' b t)
-
-unfold
-let strengthen
-  (#t: Type0)
-  (p: weak_parser t)
-: Pure (parser t)
-  (requires (no_lookahead t p))
-  (ensures (fun _ -> True))
-= let p' : bare_parser t = p in
-  (p' <: parser t)
 
 (** A parser that always consumes all its input *)
 
@@ -255,3 +227,104 @@ let consumes_all
     let (Some (_, len)) = parse p b in
     Seq.length b == len
   )
+
+(** Parsing data of constant size *)
+
+let is_constant_size_parser
+  (sz: nat)
+  (#t: Type0)
+  (f: bare_parser t)
+: GTot Type0
+= forall (s: bytes32) .
+  Some? (f s) ==> (
+    let (_, consumed) = Some?.v (f s) in
+    sz == (consumed <: nat)
+  )
+
+let is_total_constant_size_parser
+  (sz: nat)
+  (#t: Type0)
+  (f: bare_parser t)
+: GTot Type0
+= forall (s: bytes32) . {:pattern (f s) }
+  (Seq.length s < sz) == (None? (f s))
+
+(* Type hierarchy *)
+
+type constant_size_parser_kind =
+  | ConstantSizeTotal
+  | ConstantSizeUnknown
+
+let constant_size_parser_kind_prop (k: constant_size_parser_kind) (sz: nat) (#t: Type0) (f: bare_parser t) : GTot Type0 =
+  match k with
+  | ConstantSizeTotal -> is_total_constant_size_parser sz f
+  | _ -> True
+
+type strong_parser_kind =
+  | StrongConstantSize: (sz: nat) -> (k: constant_size_parser_kind) -> strong_parser_kind
+  | StrongUnknown
+
+let strong_parser_kind_prop (k: strong_parser_kind) (#t: Type0) (f: bare_parser t) : GTot Type0 =
+  match k with
+  | StrongConstantSize sz k' ->
+    is_constant_size_parser sz f /\
+    constant_size_parser_kind_prop k' sz f
+  | _ -> True
+
+type parser_kind =
+  | ParserStrong: (k' : strong_parser_kind) -> parser_kind
+  | ParserConsumesAll
+  | ParserUnknown
+
+let parser_kind_prop (k: parser_kind) (#t: Type0) (f: bare_parser t) : GTot Type0 =
+  match k with
+  | ParserStrong k' ->
+    no_lookahead f /\
+    strong_parser_kind_prop k' f
+  | ParserConsumesAll ->
+    consumes_all f
+  | _ -> True
+
+let parser
+  (k: parser_kind)
+  (t: Type0)
+: Tot Type0
+= (f: bare_parser t { no_lookahead_weak f /\ injective f /\ parser_kind_prop k f } )
+
+let is_weaker_than
+  (k1 k2: parser_kind)
+: GTot Type0
+= match k1 with
+  | ParserUnknown -> True
+  | ParserConsumesAll -> k2 == ParserConsumesAll
+  | ParserStrong k1s ->
+    begin match k2 with
+    | ParserStrong k2s ->
+      begin match k1s with
+      | StrongUnknown -> True
+      | StrongConstantSize sz1 k1c ->
+	begin match k2s with
+	| StrongConstantSize sz2 k2c ->
+	  sz1 == sz2 /\
+	  begin match k1c with
+	  | ConstantSizeUnknown -> True
+	  | ConstantSizeTotal -> k2c == ConstantSizeTotal
+	  end
+	| _ -> False
+	end
+      end
+    | _ -> False
+    end
+
+inline_for_extraction
+let weaken (k1: parser_kind) (#k2: parser_kind) (#t: Type0) (p2: parser k2 t) : Pure (parser k1 t)
+  (requires (k1 `is_weaker_than` k2))
+  (ensures (fun _ -> True))
+= let p : bare_parser t = p2 in
+  p
+
+inline_for_extraction
+let strengthen (k: parser_kind) (#t: Type0) (f: bare_parser t) : Pure (parser k t)
+  (requires (no_lookahead_weak f /\ injective f /\ parser_kind_prop k f))
+  (ensures (fun _ -> True))
+= f
